constant time mostly done

proofs/fstar/extraction-edited/Libcrux.Kem.Kyber.Constant_time_ops.fst
@@ -4,66 +4,160 @@ open Core
 open FStar.Mul
 
 let is_non_zero (value: u8) =
+  let orig_value = value in
   let value:u16 = cast (value <: u8) <: u16 in
   let result:u16 =
     ((value |. (Core.Num.impl__u16__wrapping_add (~.value <: u16) 1us <: u16) <: u16) >>! 8l <: u16) &.
     1us
   in
   let res = cast (result <: u16) <: u8 in
-  admit();
-  res
+  if v orig_value = 0 then  (
+    assert(value == zero);
+    lognot_lemma value;
+    assert((~.value +. 1us) == zero);
+    assert((Core.Num.impl__u16__wrapping_add (~.value <: u16) 1us <: u16) == zero);
+    logor_lemma value zero;
+    assert((value |. (Core.Num.impl__u16__wrapping_add (~.value <: u16) 1us <: u16) <: u16) == value);
+    assert (result == ((value >>! 8l) &. 1us));
+    assert ((v value / pow2 8) == 0);
+    logand_lemma 1us zero;
+    assert (result == 0us);
+    res)
+  else (// need some get_bit reasoning here
+    assert (v value <> 0);
+    assume (v (~.value) = pow2 16 - 1 - v value);
+    assert (v (~.value) + 1 = pow2 16 - v value);
+    assert (v (value) <= pow2 8 - 1);
+    assert ((v (~.value) + 1) = (pow2 16 - pow2 8) + (pow2 8 - v value));
+    assert ((v (~.value) + 1) = (pow2 8 - 1) * pow2 8 + (pow2 8 - v value));
+    assert ((v (~.value) + 1)/pow2 8 = (pow2 8 - 1));
+    admit() 
+  )
 
-let compare_ciphertexts_in_constant_time (v_CIPHERTEXT_SIZE: usize) (lhs rhs: t_Slice u8) =
+let compare_ciphertexts_in_constant_time v_CIPHERTEXT_SIZE lhs rhs =
   let _:Prims.unit = () <: Prims.unit in
   let _:Prims.unit = () <: Prims.unit in
   let (r: u8):u8 = 0uy in
+  [@ inline_let]
+  let inv = fun (acc:u8) (i:usize) ->
+    v i <= v v_CIPHERTEXT_SIZE /\
+   (if (Seq.slice lhs 0 (v i) = Seq.slice rhs 0 (v i)) then
+      acc == 0uy
+    else ~ (acc == 0uy))
+  in
   let r:u8 =
-    Core.Iter.Traits.Iterator.f_fold (Core.Iter.Traits.Collect.f_into_iter ({
+    Rust_primitives.Iterators.foldi_range #_ #u8  #inv {
               Core.Ops.Range.f_start = sz 0;
               Core.Ops.Range.f_end = v_CIPHERTEXT_SIZE
             }
-            <:
-            Core.Ops.Range.t_Range usize)
-        <:
-        Core.Ops.Range.t_Range usize)
       r
       (fun r i ->
           let r:u8 = r in
           let i:usize = i in
-          r |. ((lhs.[ i ] <: u8) ^. (rhs.[ i ] <: u8) <: u8) <: u8)
+          let nr = r |. ((lhs.[ i ] <: u8) ^. (rhs.[ i ] <: u8) <: u8) <: u8 in
+          if r =. 0uy then (
+            if (Seq.index lhs (v i) = Seq.index rhs (v i)) then (
+               logxor_lemma (Seq.index lhs (v i)) (Seq.index rhs (v i));
+               assert (((lhs.[ i ] <: u8) ^. (rhs.[ i ] <: u8) <: u8) = zero);
+               logor_lemma r ((lhs.[ i ] <: u8) ^. (rhs.[ i ] <: u8) <: u8);
+               assert (nr = r);
+               assert (forall j. Seq.index (Seq.slice lhs 0 (v i)) j == Seq.index lhs j);
+               assert (forall j. Seq.index (Seq.slice rhs 0 (v i)) j == Seq.index rhs j);
+               eq_intro (Seq.slice lhs 0 (v i + 1)) (Seq.slice rhs 0 (v i + 1));
+               nr
+            )
+            else (
+               logxor_lemma (Seq.index lhs (v i)) (Seq.index rhs (v i));
+               assert (((lhs.[ i ] <: u8) ^. (rhs.[ i ] <: u8) <: u8) <>  zero);
+               logor_lemma r ((lhs.[ i ] <: u8) ^. (rhs.[ i ] <: u8) <: u8);
+               assert (v nr > 0);
+               assert (Seq.index (Seq.slice lhs 0 (v i+1)) (v i) <> 
+                       Seq.index (Seq.slice rhs 0 (v i+1)) (v i));
+               assert (Seq.slice lhs 0 (v i+1) <> Seq.slice rhs 0 (v i + 1));
+               nr
+            )
+          ) else (
+            logor_lemma r ((lhs.[ i ] <: u8) ^. (rhs.[ i ] <: u8) <: u8);
+            assert (v nr >= v r);
+            assert (Seq.slice lhs 0 (v i) <> Seq.slice rhs 0 (v i));
+            if (Seq.slice lhs 0 (v i+1) = Seq.slice rhs 0 (v i + 1)) then
+              (assert (forall j. j < v i + 1 ==> Seq.index (Seq.slice lhs 0 (v i+1)) j == Seq.index (Seq.slice rhs 0 (v i+1)) j);
+               eq_intro (Seq.slice lhs 0 (v i)) (Seq.slice rhs 0 (v i));
+               assert(False))
+            else nr
+          )
+     )
   in
   let res = is_non_zero r in
-  admit();
   res
 
+#push-options "--ifuel 0 --z3rlimit 50"
 let select_shared_secret_in_constant_time (lhs rhs: t_Slice u8) (selector: u8) =
   let _:Prims.unit = () <: Prims.unit in
   let _:Prims.unit = () <: Prims.unit in
   let mask:u8 = Core.Num.impl__u8__wrapping_sub (is_non_zero selector <: u8) 1uy in
+  assert (if selector = 0uy then mask = ones else mask = zero);
+  lognot_lemma mask;
+  assert (if selector = 0uy then ~.mask = zero else ~.mask = ones);
   let out:t_Array u8 (sz 32) = Rust_primitives.Hax.repeat 0uy (sz 32) in
+  [@ inline_let]
+  let inv = fun (acc:t_Array u8 (sz 32)) (i:usize) ->
+    v i <= 32 /\
+   (forall j. j < v i ==> (if (selector =. 0uy) then Seq.index acc j == Seq.index lhs j else Seq.index acc j == Seq.index rhs j)) /\
+   (forall j. j >= v i ==> Seq.index acc j == 0uy)
+  in
   let out:t_Array u8 (sz 32) =
-    Core.Iter.Traits.Iterator.f_fold (Core.Iter.Traits.Collect.f_into_iter ({
+    Rust_primitives.Iterators.foldi_range #_ #(t_Array u8 (sz 32))  #inv {
               Core.Ops.Range.f_start = sz 0;
               Core.Ops.Range.f_end = Libcrux.Kem.Kyber.Constants.v_SHARED_SECRET_SIZE
             }
-            <:
-            Core.Ops.Range.t_Range usize)
-        <:
-        Core.Ops.Range.t_Range usize)
       out
       (fun out i ->
           let out:t_Array u8 (sz 32) = out in
-          let i:usize = i in
-          Rust_primitives.Hax.Monomorphized_update_at.update_at_usize out
-            i
+          assert ((out.[ i ] <: u8) = 0uy);
+          let outi = 
             ((out.[ i ] <: u8) |.
               (((lhs.[ i ] <: u8) &. mask <: u8) |. ((rhs.[ i ] <: u8) &. (~.mask <: u8) <: u8)
                 <:
                 u8)
               <:
-              u8)
+              u8) in
+          if (selector = 0uy) then (
+            logand_lemma (lhs.[ i ] <: u8) mask;
+            assert (((lhs.[ i ] <: u8) &. mask <: u8) == (lhs.[ i ] <: u8));
+            logand_lemma (rhs.[ i ] <: u8) (~.mask);
+            assert (((rhs.[ i ] <: u8) &. (~.mask <: u8) <: u8) == zero);
+            logor_lemma ((lhs.[ i ] <: u8) &. mask <: u8) ((rhs.[ i ] <: u8) &. (~.mask <: u8) <: u8);
+            assert ((((lhs.[ i ] <: u8) &. mask <: u8) |. ((rhs.[ i ] <: u8) &. (~.mask <: u8) <: u8) <: u8) == (lhs.[ i ] <: u8));
+            logor_lemma (out.[ i ] <: u8) (lhs.[ i ] <: u8);
+            assert (((out.[ i ] <: u8) |. (((lhs.[ i ] <: u8) &. mask <: u8) |. ((rhs.[ i ] <: u8) &. (~.mask <: u8) <: u8) <: u8) <: u8) == (lhs.[ i ] <: u8));
+            assert (outi = (lhs.[ i ] <: u8))
+          )
+          else (
+            logand_lemma (lhs.[ i ] <: u8) mask;
+            assert (((lhs.[ i ] <: u8) &. mask <: u8) == zero);
+            logand_lemma (rhs.[ i ] <: u8) (~.mask);
+            assert (((rhs.[ i ] <: u8) &. (~.mask <: u8) <: u8) == (rhs.[ i ] <: u8));
+            logor_lemma (rhs.[ i ] <: u8) zero;
+            assert ((logor zero (rhs.[ i ] <: u8)) == (rhs.[ i ] <: u8));
+            assert ((((lhs.[ i ] <: u8) &. mask <: u8) |. ((rhs.[ i ] <: u8) &. (~.mask <: u8) <: u8)) == (rhs.[ i ] <: u8));
+            logor_lemma (out.[ i ] <: u8) (rhs.[ i ] <: u8);
+            assert (((out.[ i ] <: u8) |. (((lhs.[ i ] <: u8) &. mask <: u8) |. ((rhs.[ i ] <: u8) &. (~.mask <: u8) <: u8) <: u8) <: u8) == (rhs.[ i ] <: u8));
+            assert (outi = (rhs.[ i ] <: u8))
+          );
+          let i:usize = i in
+          Rust_primitives.Hax.Monomorphized_update_at.update_at_usize out
+            i
+            outi
           <:
           t_Array u8 (sz 32))
   in
-  admit();
-  out
+  if (selector =. 0uy) then (
+    eq_intro out lhs;
+    out
+  )
+  else (
+    eq_intro out rhs;
+    out
+  )
+#pop-options
